Patterns.thy
@@ -1,0 +1,7 @@
+theory Patterns
+  imports
+Always
+Constrained_Until
+begin
+
+end
